compiler/src/ExprImp.v
@@ -67,10 +67,10 @@ Section ExprImp1.
         | cmd.skip => Some (st, m)
         | cmd.call binds fname args =>
           'Some (params, rets, fbody) <- map.get e fname;
-          'Some argvs <- option_all (List.map (eval_expr m st) args);
+          'Some argvs <- List.option_all (List.map (eval_expr m st) args);
           'Some st0 <- map.putmany_of_list params argvs map.empty;
           'Some (st1, m') <- eval_cmd f st0 m fbody;
-          'Some retvs <- option_all (List.map (map.get st1) rets);
+          'Some retvs <- List.option_all (List.map (map.get st1) rets);
           'Some st' <- map.putmany_of_list binds retvs st;
           Some (st', m')
         | cmd.interact _ _ _ => None (* unsupported *)
@@ -187,10 +187,10 @@ Section ExprImp1.
       eval_cmd (S f) st m1 (cmd.call binds fname args) = Some p2 ->
       exists params rets fbody argvs st0 st1 m' retvs st',
         map.get e fname = Some (params, rets, fbody) /\
-        option_all (List.map (eval_expr m1 st) args) = Some argvs /\
+        List.option_all (List.map (eval_expr m1 st) args) = Some argvs /\
         map.putmany_of_list params argvs map.empty = Some st0 /\
         eval_cmd f st0 m1 fbody = Some (st1, m') /\
-        option_all (List.map (map.get st1) rets) = Some retvs /\
+        List.option_all (List.map (map.get st1) rets) = Some retvs /\
         map.putmany_of_list binds retvs st = Some st' /\
         p2 = (st', m').
     Proof. inversion_lemma. Qed.
